

CSE400 – Fundamentals of Probability in Computing

Lecture 11: Transformation of Random Variables

Dhaval Patel, PhD (Associate Professor)
SEAS – Ahmedabad University, Ahmedabad, Gujarat, India

February 10, 2026

Overview / Outline (as in lecture)

1. Transformation of Random Variables

Learning of transformation techniques for random variables.

2. Function of Two Random Variables

Joint transformations and derived distributions.

3. Illustrative Example

Detailed derivation for the case: $Z = X + Y$.

1 Definitions & Notation

- Random variable (RV): X, Y, Z .
- Transformation (single RV): $Y = g(X)$.
- CDF of a RV X : $F_X(x) = \Pr(X \leq x)$.
- PDF of a continuous RV X : $f_X(x)$, with the relationship

$$f_X(x) = \frac{d}{dx}F_X(x) \quad (\text{when differentiable}).$$

- Inverse mapping (when it exists): $x = g^{-1}(y)$.

2 Assumptions / Constraints (as used in the lecture derivations)

- The PDF of the original RV (e.g., $f_X(x)$) is assumed to be known *a priori*.
- For the single-variable transformation method shown:
 - $g(\cdot)$ is **monotonic** (lecture separates cases: *+ve* / increasing vs *-ve* / decreasing).
 - $g^{-1}(\cdot)$ exists on the relevant range.
 - Differentiation steps assume the needed derivatives exist.
- If a detail/condition is not explicitly provided beyond the above, it is **Not specified in the provided context**.

3 Main Results / Theorems (with conditions)

3.1 Single RV transformation: $Y = g(X)$ (monotonic g)

Step S1 (CDF method).

Case 1: g is increasing (“+ve” monotone)

$$F_Y(y) = \Pr(Y \leq y) \quad (1)$$

$$= \Pr(g(X) \leq y) \quad (2)$$

$$= \Pr(X \leq g^{-1}(y)) \quad (3)$$

$$= F_X(g^{-1}(y)). \quad (4)$$

Case 2: g is decreasing (“-ve” monotone)

$$F_Y(y) = \Pr(Y \leq y) \quad (5)$$

$$= \Pr(g(X) \leq y) \quad (6)$$

$$= \Pr(X \geq g^{-1}(y)) \quad (7)$$

$$= 1 - F_X(g^{-1}(y)). \quad (8)$$

Step S2 (Differentiate to obtain PDF).

Increasing case Differentiate $F_Y(y) = F_X(g^{-1}(y))$ w.r.t. y :

$$f_Y(y) = \frac{d}{dy} F_Y(y) \quad (9)$$

$$= \frac{d}{dy} [F_X(g^{-1}(y))] \quad (10)$$

$$= f_X(g^{-1}(y)) \cdot \frac{d}{dy} [g^{-1}(y)]. \quad (11)$$

Let $x = g^{-1}(y)$. Then $\frac{dx}{dy} = \frac{d}{dy} g^{-1}(y)$, so

$$f_Y(y) = f_X(x) \left| \frac{dx}{dy} \right| \quad \text{with } x = g^{-1}(y).$$

Decreasing case Starting from $F_Y(y) = 1 - F_X(g^{-1}(y))$:

$$f_Y(y) = \frac{d}{dy} F_Y(y) \quad (12)$$

$$= -f_X(g^{-1}(y)) \cdot \frac{d}{dy} [g^{-1}(y)]. \quad (13)$$

Taking absolute value (as emphasized in the lecture’s boxed formula), the unified form is

$$f_Y(y) = f_X(x) \left| \frac{dx}{dy} \right| \quad \text{with } x = g^{-1}(y).$$

Step S3 (Change the limits / support).

The valid range of y is obtained by mapping the support of x through $y = g(x)$ (lecture notes: “change the limits for Y ”).

3.2 Equivalent boxed formula shown in the lecture

Using $\left| \frac{dx}{dy} \right| = \frac{1}{\left| \frac{dy}{dx} \right|}$ (when derivatives exist),

$$f_Y(y) = \frac{f_X(x)}{\left| \frac{dy}{dx} \right|} \Big|_{x=g^{-1}(y)}$$

This is the boxed relationship displayed in the lecture.

4 Proofs / Derivations (step-by-step, as in lecture)

4.1 Derivation structure for $Y = g(X)$

The lecture's derivation proceeds in the following explicit sequence:

S1: Compute $F_Y(y) = \Pr(Y \leq y)$ and rewrite the event in terms of X using monotonicity and the inverse g^{-1} .

S2: Differentiate $F_Y(y)$ w.r.t. y to obtain $f_Y(y)$, applying the chain rule.

S3: Determine the correct support/range for y by transforming the original x -limits through $y = g(x)$.

4.2 Two-RV function setup used for the example $Z = X + Y$

The lecture sets up the CDF of Z via a region in the (x, y) -plane:

$$F_Z(z) = \Pr(Z \leq z) \tag{14}$$

$$= \Pr(X + Y \leq z). \tag{15}$$

Using the joint PDF $f_{X,Y}(x, y)$, the probability is written as a double integral over the region

$$\{(x, y) : x + y \leq z\}.$$

One explicit “vertical strip” form written in the lecture is:

$$F_Z(z) = \int_{x=-\infty}^{\infty} \int_{y=-\infty}^{z-x} f_{X,Y}(x, y) dy dx.$$

(An equivalent “horizontal strip” order is implied by the lecture's annotation about vertical/horizontal swapping, but any further simplification is **Not specified in the provided context.**)

Then, to obtain the PDF:

$$f_Z(z) = \frac{d}{dz} F_Z(z).$$

Any closed-form $f_Z(z)$ beyond this setup depends on additional assumptions/distributions, which are listed as sub-questions in the lecture (see Worked Examples).

5 Worked Examples (step-by-step)

5.1 Example 1: $X \sim \text{Uniform}(-1, 1)$, $Y = g(X) = \sin\left(\frac{\pi X}{2}\right)$

Given (as written in the lecture):

$$f_X(x) = \begin{cases} \frac{1}{2}, & -1 < x < 1, \\ 0, & \text{otherwise.} \end{cases} \quad Y = \sin\left(\frac{\pi X}{2}\right).$$

Step 1: Invert the transformation.

From $y = \sin\left(\frac{\pi x}{2}\right)$,

$$x = \frac{2}{\pi} \sin^{-1}(y).$$

Step 2: Compute the derivative factor.

$$\frac{dx}{dy} = \frac{2}{\pi} \cdot \frac{1}{\sqrt{1-y^2}}.$$

Step 3: Apply the transformation formula. Using $f_Y(y) = f_X(x) \left| \frac{dx}{dy} \right|$ with $x = \frac{2}{\pi} \sin^{-1}(y)$:

$$f_Y(y) = \frac{1}{2} \cdot \left| \frac{2}{\pi} \cdot \frac{1}{\sqrt{1-y^2}} \right| \quad (16)$$

$$= \frac{1}{\pi \sqrt{1-y^2}}. \quad (17)$$

Step 4: Determine the support (change limits).

Lecture maps endpoints:

$$x = -1 \Rightarrow y = \sin\left(-\frac{\pi}{2}\right) = -1, \quad x = 1 \Rightarrow y = \sin\left(\frac{\pi}{2}\right) = 1.$$

Hence,

$$f_Y(y) = \begin{cases} \frac{1}{\pi \sqrt{1-y^2}}, & -1 < y < 1, \\ 0, & \text{otherwise.} \end{cases}$$

5.2 Example 2 (illustrative setup): $Z = X + Y$

The lecture explicitly states the following items to find/prove (no full solutions shown beyond the CDF-region setup):

- (i) Find the PDF of Z , $f_Z(z)$.
- (ii) Find $f_Z(z)$ if X and Y are independent.
- (iii) Let $X \sim N(0, 1)$ and $Y \sim N(0, 1)$. Prove that $Z \sim N(0, 2)$.
- (iv) If X and Y are exponential distributed RVs with parameter λ , find $f_Z(z)$.

Derivation shown (CDF setup):

$$F_Z(z) = \Pr(Z \leq z) \quad (18)$$

$$= \Pr(X + Y \leq z) \quad (19)$$

$$= \iint_{x+y \leq z} f_{X,Y}(x, y) dx dy \quad (20)$$

$$= \int_{-\infty}^{\infty} \int_{-\infty}^{z-x} f_{X,Y}(x, y) dy dx. \quad (21)$$

Further evaluation for cases (ii)–(iv) is **Not specified in the provided context** beyond listing these tasks.

Summary of Key Takeaways (only from context)

- To find the distribution of a transformed RV $Y = g(X)$ (with monotonic g), the lecture uses the **CDF method** followed by differentiation.
- For monotonic transformations, the resulting PDF uses the absolute derivative factor:

$$f_Y(y) = f_X(g^{-1}(y)) \left| \frac{d}{dy} g^{-1}(y) \right| \quad \text{equivalently} \quad f_Y(y) = \frac{f_X(x)}{\left| \frac{dy}{dx} \right|} \Big|_{x=g^{-1}(y)}.$$

- The support of the new RV must be obtained by **changing limits** (mapping x -range through $y = g(x)$).
- For $Z = X + Y$, the lecture sets up $F_Z(z) = \Pr(X + Y \leq z)$ as a **double integral over the half-plane** $x + y \leq z$ using $f_{X,Y}(x, y)$, and then uses $f_Z(z) = \frac{d}{dz} F_Z(z)$.